Added new h lemma, changed definition of EvenStream and finished proof for bot assumption #53

untimed/CaseStudy/EvenAutomaton.thy
@@ -97,30 +97,48 @@ by (metis option.simps(3))
 
 lift_definition EvenAutomatonAutomaton :: "(EvenAutomatonState, EvenAutomaton event) automaton" is 
   "(evenAutomatonTransition, State Even 0,(tsynbOneTick c2), {c1}, {c2})"
-  sorry
-
+  apply(rule automaton_wellI,simp)
+proof-
+  fix s::EvenAutomatonState
+  fix f::"channel \<Rightarrow> EvenAutomaton event option"
+  show "dom f = {c1} \<Longrightarrow> ubDom\<cdot>(snd (evenAutomatonTransition (s, f))) = {c2}"
+    apply(subst evenAutomatonTransition.pinduct, simp_all)
+    sorry
+qed
+  
 definition EvenAutomatonSPF :: "EvenAutomaton event SPF" where
 "EvenAutomatonSPF = H EvenAutomatonAutomaton"
 
+lemma evenStreamBundle_well[simp]:assumes "sdom\<cdot>s \<subseteq> ctype c" shows "ubWell ([c \<mapsto> s::EvenAutomaton event stream])"
+by(simp add: ubWell_def usclOkay_stream_def assms)
+
 
 definition EvenStream::"EvenAutomatonState \<Rightarrow> EvenAutomaton event stream \<rightarrow> EvenAutomaton event stream" where
-"EvenStream state \<equiv> (\<Lambda> st. sdrop 1\<cdot>((EvenAutomatonSPF \<rightleftharpoons> (Abs_ubundle [c1 \<mapsto> (\<up>( Msg (A (getSum state))) \<bullet> st)])). c2))"
+"EvenStream state \<equiv> (\<Lambda> s. ((h EvenAutomatonAutomaton state) \<rightleftharpoons> (Abs_ubundle [c1 \<mapsto> s])) . c2)"
 
 fun evenMakeSubstate :: "bool \<Rightarrow> EvenAutomatonSubstate" where
 "evenMakeSubstate True = Even" | 
 "evenMakeSubstate False = Odd"
 
-lemma evenStream_insert:"EvenStream state\<cdot>s = sdrop 1\<cdot>((EvenAutomatonSPF \<rightleftharpoons> (Abs_ubundle [c1 \<mapsto> (\<up>( Msg (A (getSum state))) \<bullet> s)])). c2)"
+lemma evenStream_insert:"EvenStream state\<cdot>s = ((h EvenAutomatonAutomaton state) \<rightleftharpoons> (Abs_ubundle [c1 \<mapsto> s])) . c2"
   apply(simp add: EvenStream_def,rule beta_cfun)
 proof(rule Cont.contI2)
-  show"monofun (\<lambda>x::EvenAutomaton event stream. sdrop (Suc (0::nat))\<cdot>((EvenAutomatonSPF \<rightleftharpoons> Abs_ubundle [c1 \<mapsto> \<up>(\<M> A (getSum state)) \<bullet> x])  .  c2))"
+  show"monofun (\<lambda>x::EvenAutomaton event stream. (h EvenAutomatonAutomaton state \<rightleftharpoons> Abs_ubundle [c1 \<mapsto> x])  .  c2)"
+   apply(rule monofunI)
     sorry
 next
   fix Y:: "nat \<Rightarrow>EvenAutomaton event stream"
   assume a1: "chain Y"
-  assume a2:"chain (\<lambda>i::nat. sdrop (Suc (0::nat))\<cdot>((EvenAutomatonSPF \<rightleftharpoons> Abs_ubundle [c1 \<mapsto> \<up>(\<M> A (getSum state)) \<bullet> Y i])  .  c2))"
-  show " sdrop (Suc (0::nat))\<cdot>((EvenAutomatonSPF \<rightleftharpoons> Abs_ubundle [c1 \<mapsto> \<up>(\<M> A (getSum state)) \<bullet> (\<Squnion>i::nat. Y i)])  .  c2) \<sqsubseteq>
-       (\<Squnion>i::nat. sdrop (Suc (0::nat))\<cdot>((EvenAutomatonSPF \<rightleftharpoons> Abs_ubundle [c1 \<mapsto> \<up>(\<M> A (getSum state)) \<bullet> Y i])  .  c2))"
+  assume a2:"chain (\<lambda>i::nat. (h EvenAutomatonAutomaton state \<rightleftharpoons> Abs_ubundle [c1 \<mapsto> Y i])  .  c2)"
+  have "\<And>i. sdom\<cdot>(Y i) \<subseteq> ctype c1"
+    sorry
+  have h1:"(Abs_ubundle [c1 \<mapsto> \<Squnion>i. Y i]) = (\<Squnion>i. Abs_ubundle [c1 \<mapsto>  Y i])"
+    sorry
+  have h2:"chain (\<lambda>i::nat. Abs_ubundle [c1 \<mapsto> Y i])"
+    sorry
+  show "(h EvenAutomatonAutomaton state \<rightleftharpoons> Abs_ubundle [c1 \<mapsto> \<Squnion>i::nat. Y i])  .  c2 \<sqsubseteq> 
+          (\<Squnion>i::nat. (h EvenAutomatonAutomaton state \<rightleftharpoons> Abs_ubundle [c1 \<mapsto> Y i])  .  c2)"
+    apply(simp add: h1, subst contlub_cfun_arg, simp add: h2)
     sorry
 qed
   
@@ -157,39 +175,12 @@ next
   case (4 s)
   then show ?case sorry
 qed*)
-    
-lemma spconc_step[simp]:
-  assumes "ubDom\<cdot>sb = ufDom\<cdot>spf"
-  shows "(spfConc sb1\<cdot>spf)\<rightleftharpoons>sb = ubConcEq sb1\<cdot>(spf\<rightleftharpoons>sb)"
-  apply(simp add: spfConc_def assms)
- sorry
-  
-lemma bot_assms: "EvenStream state\<cdot>\<bottom> = \<bottom>"
-  apply(simp add: evenStream_insert EvenAutomatonSPF_def H_def getInitialOutput_def EvenAutomatonAutomaton.rep_eq)
-  apply(subst spconc_step, simp add: EvenAutomatonAutomaton.rep_eq getDom_def ubDom_def)
-sorry
       
-(*  
-lemma type_assms: "tsynDom\<cdot>(xs::EvenAutomaton event stream) \<subseteq> range A"
-  proof(induction rule: tsyn_ind [of _xs])
-    case 1
-    then show ?case 
-      by simp
-  next
-    case 2
-    then show ?case
-      by(simp add: tsyndom_insert)
-  next
-    case (3 a s)
-    then show ?case
-      apply(simp add: tsyndom_insert, auto)
-      apply(cases "a")
-      apply simp
-      sorry
-  next
-    case (4 s)
-    then show ?case
-      by(simp add: tsyndom_insert)
-  qed*)
+lemma bot_assms: "EvenStream state\<cdot>\<bottom> = \<bottom>"
+  apply(simp add: evenStream_insert)
+  apply(subst h_bottom, simp add: getDom_def EvenAutomatonAutomaton.rep_eq ubDom_def)
+  apply(simp add: getDom_def EvenAutomatonAutomaton.rep_eq)
+  apply(subst ubgetch_ubrep_eq, auto)
+  by(simp add: getRan_def EvenAutomatonAutomaton.rep_eq ubclLeast_ubundle_def)
     
 end
